Simple Data: finish most of Preservation

proof/Simple_Data/EsJudge.v
@@ -1,4 +1,5 @@
 
+Require Import TyJudge.
 Require Export Exp.
 Require Export SubstExpExp.
 
@@ -57,17 +58,64 @@ Inductive exp_ctx : (exp -> exp) -> Prop :=
 (** * Utilities for evaluation *)
 
 (* Get the alternative body that matches a given constructor. *)
-Fixpoint getAltExp (dc: datacon) (alts: list alt) {struct alts} 
-                   : option exp :=
+Fixpoint getAlt (dc: datacon) (alts: list alt) {struct alts} 
+                : option alt :=
  match alts with 
  |  nil  => None
 
- |  AAlt dc' _ x :: alts'
+ |  AAlt dc' tsArgs x :: alts'
  => if datacon_beq dc dc'
-     then Some x
-     else getAltExp dc alts'
+     then Some (AAlt dc' tsArgs x)
+     else getAlt dc alts'
  end.
 
+
+Lemma getAltExp_hasAlt
+ :  forall dc alt alts
+ ,  getAlt dc alts = Some alt
+ -> In alt alts.
+Proof.
+ intros.
+ induction alts.
+  false.
+  destruct a as [dc' tsArgs x].
+  simpl in H.
+  breaka (datacon_beq dc dc').
+   inverts H.
+    assert (dc = dc'). admit. (* ok datacon_beq *)
+    subst. clear HeqX.
+    simpl. auto.
+
+   simpl. right. eauto.
+Qed.
+
+
+Lemma getAltExp_good
+ :  forall ds te tPat tResult alts dc tsArgs x
+ ,  Forall (fun a => TYPEA ds te a tPat tResult) alts
+ -> In (AAlt dc tsArgs x) alts
+ -> TYPE ds (te ++ envOfList tsArgs) x tResult.
+Proof.
+ intros.
+ rewrite Forall_forall in H.
+ eapply H in H0. inverts H0. eauto.
+Qed.
+
+
+Lemma getAltExp_inAlts
+ :  forall ds te tResult tCon alts dc tsArgs x1 x2
+ ,  TYPE ds te (XCase x1 alts) tResult
+ -> getDataDef dc ds   = Some (DefData dc tsArgs tCon)
+ -> getAlt     dc alts = Some (AAlt    dc tsArgs x2)
+ -> TYPE ds (te ++ envOfList tsArgs) x2 tResult.
+Proof.
+ intros.
+ inverts keep H.
+ lets HA:  getAltExp_hasAlt H1.
+ lets HXT: getAltExp_good H5 HA.
+ auto.
+Qed.
+ 
 
 (********************************************************************)
 (** * Single Small Step Evaluation *)
@@ -90,9 +138,9 @@ Inductive STEP : exp -> exp -> Prop :=
            (substX 0 v2 x12)
 
  | EsCaseAlt
-   :  forall dc vs alts x
+   :  forall dc vs tsArgs alts x
    ,  Forall value vs
-   -> getAltExp dc alts = Some x
+   -> getAlt dc alts = Some (AAlt dc tsArgs x)
    -> STEP (XCase (XCon dc vs) alts)
            (substXs 0 vs x).
 
