proof/Simple_Data/Preservation.v
@@ -4,6 +4,23 @@ Require Import EsJudge.
 Require Import SubstExpExp.
 
 
+Lemma getAlt_matches_dataDef
+ :  forall ds te tCon tResult alts dc x tsArgs tsArgs'
+ ,  Forall (fun alt => TYPEA ds te alt tCon tResult) alts 
+ -> getDataDef dc ds = Some (DefData dc tsArgs  tCon)
+ -> getAlt dc alts   = Some (AAlt    dc tsArgs' x)
+ -> tsArgs = tsArgs'.
+Proof.
+ intros.
+ rewrite Forall_forall in H.
+ lets D: getAltExp_hasAlt H1.
+ apply H in D.
+ inverts D.
+ rewrite H0 in H9.
+ inverts H9. auto.
+Qed.
+ 
+
 (* When a well typed expression transitions to the next state
    then its type is preserved.
  *)
@@ -39,8 +56,16 @@ Proof.
   eapply subst_value_value; eauto.
 
  Case "EsCaseAlt".
-  inverts HT. inverts H5.
-  (* TODO: finish this. need subst for list of exps *)
+  inverts keep HT. inverts H3.
+  eapply subst_value_value_list.
+  eauto.
+  eapply getAltExp_inAlts.
+   eauto.
+   eauto. auto.
+   assert (tsArgs = tsArgs0).
+   lets D: getAlt_matches_dataDef H4 H9 H0. auto.
+   rewrite <- H1.
+   auto.
 Qed.
 
 
